src/program_proof/pav/server.v
@@ -10,15 +10,58 @@ From Perennial.base_logic Require Import ghost_map.
 Module hashChain.
 Record t :=
   mk {
+    data: list (list w8);
     links: list (list w8);
   }.
 
 Section local_defs.
 Context `{!heapGS Σ}.
 Definition own ptr obj : iProp Σ :=
-  ∃ h,
-  chainSepNone.hashes_to h ∗
-  own_Slice2D ptr (DfracOwn 1) (h :: obj.(links)).
+  ∃ sl_links h,
+  "Hlinks" ∷ ptr ↦[hashChain :: "links"] (slice_val sl_links) ∗
+  "#Hinit" ∷ chainSepNone.hashes_to h ∗
+  "Hown" ∷ own_Slice2D sl_links (DfracOwn 1) (h :: obj.(links)) ∗
+  "#Hbinds" ∷ ([∗ list] epoch ↦ d; l ∈ obj.(data); obj.(links),
+    is_hash (chainSepSome.encodesF (chainSepSome.mk epoch ((h :: obj.(links)) !!! epoch) d)) l).
+
+Definition wp_put ptr obj sl_data b d0 :
+  {{{
+    "Hchain" ∷ own ptr obj ∗
+    "Hdata" ∷ own_slice_small sl_data byteT d0 b
+  }}}
+  hashChain__put #ptr (slice_val sl_data)
+  {{{
+    (* don't write out new links since that's implied from the bindings. *)
+    new_links, RET #();
+    "Hchain" ∷ own ptr (mk (obj.(data) ++ [b]) new_links)
+  }}}.
+Proof. Admitted.
+
+(*
+TODO:
+it seems more intuitive to give back a resource that logically commits
+to all the data before it.
+a binding is a more low-level resource.
+it only talks about the prev data.
+something like is_tree_dig, which ties together the data entries along with the commitment.
+but here there's a bit of peeling the black box, as we should be able
+to reconstruct a valid link from its composing vals.
+the resource itself could just be the Hbind big sep,
+with convenient lemmas around it for doing the most common ops.
+*)
+Definition wp_getLink ptr obj (len : w64) :
+  uint.nat len ≤ length obj.(data) →
+  {{{
+    "Hchain" ∷ own ptr obj
+  }}}
+  hashChain__getLink #ptr #len
+  {{{
+    sl_link h, RET (slice_val sl_link);
+    "Hchain" ∷ own ptr obj ∗
+    "#Hinit" ∷ chainSepNone.hashes_to h ∗
+    "#Hlink" ∷ own_slice_small sl_link byteT DfracDiscarded ((h :: obj.(links)) !!! (uint.nat len))
+  }}}.
+Proof. Admitted.
 End local_defs.
 End hashChain.
 
@@ -34,34 +77,39 @@ Record t :=
 Section local_defs.
 Context `{!heapGS Σ, !mono_listG (list w8) Σ, !mono_listG gname Σ, !ghost_mapG Σ (list w8) (list w8)}.
 
-Definition my_inv γmonoLinks γmonoTrees : iProp Σ :=
-  ∃ links γtrees trees updates prevLinks digs,
-  "#Hbinds" ∷ ([∗ list] epoch ↦ xy; link ∈ (zip prevLinks digs); links,
-    is_hash (chainSepSome.encodesF (chainSepSome.mk epoch xy.1 xy.2)) link) ∗
-  "Hlinks" ∷ mono_list_auth_own γmonoLinks (1/2) links ∗
-  "Htree_views" ∷ ([∗ list] γtr; tr ∈ γtrees; (trees ++ [updates]),
-    ghost_map_auth γtr (1/2) tr) ∗
-  "HmonoTrees" ∷ mono_list_auth_own γmonoTrees (1/2) γtrees ∗
-  "#Hdigs" ∷ ([∗ list] tr; dig ∈ trees; digs, isTreeDig tr dig).
+(*
+   things getting a bit too abstract.
+   in put func, how will client prove link sigpred?
+   client needs to produce binding as well as mono_idx's.
 
+   we have prev2Link, which comes directly from links and therefore
+   has mono_idx resource along with it.
+
+   from global inv, access the binding for the prev link.
+   there will be an existential link.
+   get the mono_idx for that link.
+   now we have all the resources we need.
+ *)
 Definition own ptr obj : iProp Σ :=
-∃ sk sl_ptr_trees (ptr_trees : list loc) trees ptr_updates (updates : gmap (list w8) (list w8)) map_sl_updates sl_chain chain sl_linkSigs linkSigs γtrees,
+∃ sk sl_ptr_trees (ptr_trees : list loc) trees ptr_updates (updates : gmap (list w8) (list w8)) map_sl_updates ptr_chain digs links sl_linkSigs linkSigs γtrees,
   "Hsk" ∷ ptr ↦[server :: "sk"] (slice_val sk) ∗
   "Hown_sk" ∷ own_sk sk (serv_sigpred obj.(γmonoLinks) obj.(γmonoTrees)) obj.(hon) ∗
-  "Hchain" ∷ ptr ↦[server :: "chain"] (slice_val sl_chain) ∗
-  "Hown_chain" ∷ hashChain.own sl_chain chain ∗
-  "HmonoLinks" ∷ mono_list_auth_own obj.(γmonoLinks) (1/2) chain.(hashChain.links) ∗
   "HlinkSigs" ∷ ptr ↦[server :: "linkSigs"] (slice_val sl_linkSigs) ∗
   "Hown_linkSigs" ∷ own_Slice2D sl_linkSigs (DfracOwn 1) linkSigs ∗
 
-  (* The latest updates. *)
+  (* hash chain. *)
+  "Hown_chain" ∷ hashChain.own ptr_chain (hashChain.mk digs links) ∗
+  "Hchain" ∷ ptr ↦[server :: "chain"] #ptr_chain ∗
+  "HmonoLinks" ∷ mono_list_auth_own obj.(γmonoLinks) (1/2) links ∗
+
+  (* latest updates. *)
   (* Exists map of slices that own the respective vals. *)
   "Hmap_sl_updates" ∷ ([∗ map] sl_bytes; bytes ∈ map_sl_updates; (kmap bytes_to_string updates),
     own_slice_small sl_bytes byteT (DfracOwn 1) bytes) ∗
   "Hown_updates" ∷ own_map ptr_updates (DfracOwn 1) map_sl_updates ∗
   "Hupdates" ∷ ptr ↦[server :: "updates"] #ptr_updates ∗
 
-  (* Tree-specific stuff. *)
+  (* merkle trees. *)
   "Htrees" ∷ ptr ↦[server :: "trees"] (slice_val sl_ptr_trees) ∗
   "Hsl_ptr_trees" ∷ own_slice_small sl_ptr_trees ptrT (DfracOwn 1) ptr_trees ∗
   "Hown_trees" ∷ ([∗ list] ptr_tr; tr ∈ ptr_trees; trees,
@@ -150,28 +198,6 @@ done.
   }
 Qed.
 
-Lemma inv_open_unify γmonoLinks links γmonoTrees γtrees trees updates :
-  mono_list_auth_own γmonoLinks (1/2) links -∗
-  mono_list_auth_own γmonoTrees (1/2) γtrees -∗
-  ([∗ list] γtr; tr ∈ γtrees; (trees ++ [updates]),
-    ghost_map_auth γtr (1/2) tr) -∗
-  inv nroot (server.my_inv γmonoLinks γmonoTrees) -∗
-  |={⊤}=>
-  ∃ prevLinks digs,
-  "#Hbinds" ∷ ([∗ list] epoch ↦ xy; link ∈ (zip prevLinks digs); links,
-    is_hash (chainSepSome.encodesF (chainSepSome.mk epoch xy.1 xy.2)) link) ∗
-  "#Hdigs" ∷ ([∗ list] tr; dig ∈ trees; digs, isTreeDig tr dig).
-Proof.
-  iIntros "Hlinks0 HmonoTrees0 Htree_views0 Hinv".
-  iInv "Hinv" as "> Hinv" "Hclose"; iNamed "Hinv".
-  iDestruct (mono_list_auth_own_agree with "Hlinks Hlinks0") as %[_ ->].
-  iDestruct (mono_list_auth_own_agree with "HmonoTrees HmonoTrees0") as %[_ ->].
-  iDestruct (sep_auth_agree with "Htree_views Htree_views0") as %?; list_simplifier.
-  iFrame "#".
-  iMod ("Hclose" with "[$]") as "_".
-  done.
-Qed.
-
 Lemma wp_server_put ptr_serv obj_serv sl_id sl_val (id val : list w8) d0 d1 :
   {{{
     "Hserv" ∷ server.valid ptr_serv obj_serv ∗
@@ -237,8 +263,8 @@ Proof.
     move: Henc => Henc_putPre.
   replace (word.add (word.sub sl_ptr_trees.(Slice.sz) (W64 1)) (W64 1)) with (sl_ptr_trees.(Slice.sz)) in Henc_putPre by ring.
 
-  (* get resources for put promise. *)
-  (* get mono_list_idx_own. *)
+  (* get resources for put / link sigpred. *)
+  (* get γtree mono_list_idx_own. *)
   iDestruct (own_slice_small_sz with "Hsl_ptr_trees") as %Hlen0.
   iDestruct (big_sepL2_length with "Hown_trees") as %Hlen1.
   iDestruct (big_sepL2_length with "Htree_views") as %Hlen2.
@@ -248,13 +274,18 @@ Proof.
   iDestruct (mono_list_idx_own_get with "[HmonoTrees]") as "#Hidx_γtree".
   2: iApply (mono_list_lb_own_get with "HmonoTrees").
   1: done.
-  (* get ghost map witness by opening invariant. *)
+  (* open invariant to get even more info. *)
   wp_apply ncfupd_wp.
   iRename "HmonoTrees" into "HmonoTrees0".
   iRename "Htree_views" into "Htree_views0".
   iInv "Hinv" as "> H" "Hclose"; iNamed "H".
   iDestruct (mono_list_auth_own_agree with "HmonoTrees HmonoTrees0") as %[_ ->].
   iDestruct (sep_auth_agree with "Htree_views Htree_views0") as %?; list_simplifier.
+  (* TODO: for link sigpred: get binding from glob inv, get prev2Link
+  from either, get prevLink from either.
+  so really critical part is getting binding. *)
+  (* extract binding for prev2Link. *)
+  (* get ghost map witness. *)
   assert ((trees ++ [updates]) !! uint.nat sl_ptr_trees.(Slice.sz) = Some updates) as Hlook1.
   { apply lookup_snoc_Some; eauto with lia. }
   iDestruct (big_sepL2_insert_acc with "Htree_views0") as "[Hmap_auth0 Hsep_close0]"; [done..|].
@@ -273,7 +304,7 @@ Proof.
   assert (uint.nat sl_ptr_trees.(Slice.sz) = length trees + 0) as H by lia;
     iEval (rewrite H insert_app_r) in "Htree_views0 Htree_views1";
     list_simplifier; clear H.
-  iMod ("Hclose" with "[$Hlinks $HmonoTrees $Htree_views1]") as "_"; [iFrame "#"|].
+  iMod ("Hclose" with "[$Hlinks $HmonoTrees $Htree_views1]") as "_"; [iFrame "%#"|].
 
   (* sign put promise. *)
   iModIntro.
@@ -295,16 +326,25 @@ Proof.
 
   (* get all the other data to be returned. *)
   wp_loadField.
-  Print serv_sigpred_link.
+  wp_apply (hashChain.wp_getLink with "Hown_chain"); [admit|].
+  iIntros (sl_link ?) "H";
+    iRename "Hchain" into "Hptr_chain";
+    iNamed "H".
+  wp_loadField.
+  remember (word.sub sl_ptr_trees.(Slice.sz) (W64 1)) as treeIdx.
+  assert (∃ ptr_tree, ptr_trees !! uint.nat treeIdx = Some ptr_tree) as [ptr_tree Hlook2] by admit.
+  wp_apply (wp_SliceGet with "[$Hsl_ptr_trees //]"); iIntros "Hsl_ptr_trees".
+  iDestruct (big_sepL2_lookup_1_some with "Hown_trees") as %[tree Htree]; [done|].
+  iDestruct (big_sepL2_lookup_acc with "Hown_trees") as "[Hown_tree Hown_trees_close]"; [done..|].
+  wp_apply (wp_Tree_Digest with "Hown_tree").
+    iIntros (sl_dig dig) "H"; iNamed "H".
+  wp_loadField.
+  iDestruct "Hown_linkSigs" as (linkSigs_dim0) "[HlinkSigs_dim0 Hown_linkSigs]".
+  assert (∃ sl_linkSig, linkSigs_dim0 !! uint.nat treeIdx = Some sl_linkSig) as [sl_linkSig Hlook3] by admit.
+  wp_apply (wp_SliceGet with "[$HlinkSigs_dim0]"); [done|]; iIntros "HlinkSigs_dim0".
   (*
-     what are we returning here?
-     at prev epoch update, we committed a new link.
-     there's an invariance that is_hash holds true for some stuff.
-     also that isTreeDig holds true, so that's what we used.
-     and direct hashChain inv is that mono_list_auth of all this.
-  *)
-  Search hashChain__getLink.
-
+     okay, now what do i need to 
+   *)
 Admitted.
 
 Lemma wp_server_updateEpoch ptr_serv obj_serv :
